grammatik/Grammatik.lean
@@ -231,3 +231,4 @@ import Grammatik.Zielsatz.Akzeptiert
 import Grammatik.Zielsatz.AkzeptiertZeuge
 import Grammatik.Zielsatz.Spec
 import Grammatik.Zielsatz.SpecProben
+import Grammatik.ZielOrtInvGrund
